test/test_flag.ml
@@ -1,0 +1,7 @@
+let _test_flag = 
+  ref true |> Tjr_global.register ~name:(__MODULE__ ^ ": test_flag")
+
+let test_flag() = !_test_flag
+
+let enable_tests() = _test_flag:=true
+let disable_tests() = _test_flag:=false
