src/d_find_ins_del/Post_monad.thy
@@ -34,44 +34,41 @@ termination iter_m
 function get_tree :: 
 "('k,'v,'leaf)leaf_ops \<Rightarrow> 
 ('k,'r,'node)node_ops \<Rightarrow> 
-('node \<Rightarrow> 'r s) \<Rightarrow> 
-('node \<Rightarrow> 'k s) \<Rightarrow> 
-('leaf \<Rightarrow> ('k * 'v) s) \<Rightarrow>
-('r,('node,'leaf)dnode,'t) store_ops \<Rightarrow> 'r \<Rightarrow> (('k,'v)tree,'t)MM" where
-"get_tree leaf_ops node_ops node2rs node2ks leaf2kvs store_ops = (% r.
+('r,('node,'leaf)dnode,'t) store_ops \<Rightarrow> 
+'r \<Rightarrow> (('k,'v)tree,'t)MM" where
+"get_tree leaf_ops node_ops store_ops = (% r.
   r |> (store_ops|>read) |> bind (% n. case n of 
-  Disk_leaf leaf \<Rightarrow> (return (Leaf(leaf2kvs leaf)))
+  Disk_leaf leaf \<Rightarrow> (return (Leaf((leaf_ops|>dbg_leaf_kvs) leaf)))
   | Disk_node n \<Rightarrow> (
     iter_m (% (ts,rs). case rs of 
       [] \<Rightarrow> return None
       | r#rs \<Rightarrow> (
-        get_tree leaf_ops node_ops node2rs node2ks leaf2kvs store_ops r |> bind (% t. 
+        get_tree leaf_ops node_ops store_ops r |> bind (% t. 
         return (Some(t#ts,rs)))))
-      ([],node2rs n)
+      ([],(node_ops|>dbg_node_krs) n |> snd)
     |> bind (% (ts,_).
-    return (Node(node2ks n,List.rev ts))))))"
+    return (Node((node_ops|>dbg_node_krs) n |> fst,List.rev ts))))))"
 apply (force)+ done
 termination get_tree
   by (force intro:FIXME)
 
 (* check tree wellformedness from a given root; note that the "min_size_t" argument may be
-overly permissive *)
+overly permissive
+
+NOTE this check_tree_at_r will always consume CPU (on the call to get_tree) even if assertions
+are disabled
+ *)
+
 definition check_tree_at_r :: "
 constants \<Rightarrow> 
 'k ord \<Rightarrow>
 ('k,'v,'leaf) leaf_ops \<Rightarrow>
 ('k,'r,'node) node_ops \<Rightarrow> 
-('node \<Rightarrow> 'r s) \<Rightarrow> 
-('node \<Rightarrow> 'k s) \<Rightarrow> 
-('leaf \<Rightarrow> ('k * 'v) s) \<Rightarrow>
 ('r,('node,'leaf)dnode,'t) store_ops \<Rightarrow>
 'r \<Rightarrow> (unit,'t)MM" where
-"check_tree_at_r cs k_cmp leaf_ops node_ops node2rs node2ks leaf2kvs store_ops r = (
-  case get_check_flag () of
-  False \<Rightarrow> return ()
-  | True \<Rightarrow> 
-    get_tree leaf_ops node_ops node2rs node2ks leaf2kvs store_ops r |> bind (% t.
-    let _ = check_true (% _. wf_tree cs (Some Small_root_node_or_leaf) k_cmp t) in
-    return ()))"
+"check_tree_at_r cs k_cmp leaf_ops node_ops store_ops r = (
+  get_tree leaf_ops node_ops store_ops r |> bind (% t.
+  let _ = assert_true (% _. wf_tree cs (Some Small_root_node_or_leaf) k_cmp t) in
+  return ()))"
 
 end
